{
 "cells": [
  {
   "cell_type": "code",
   "execution_count": 5,
   "id": "108b17fc",
   "metadata": {},
   "outputs": [],
   "source": [
    "import pandas as pd \n",
    "import os \n",
    "\n",
    "from transformers import AutoModelForCausalLM, AutoTokenizer\n",
    "from datasets import load_dataset\n",
    "\n",
    "import seaborn as sns\n",
    "\n",
    "from datasets import load_dataset\n",
    "import numpy as np\n",
    "import json"
   ]
  },
  {
   "cell_type": "code",
   "execution_count": 2,
   "id": "56a7421e",
   "metadata": {
    "scrolled": true
   },
   "outputs": [
    {
     "data": {
      "text/plain": [
       "'/home/al2644/research/codebase/reasoning/perturb-r/notebook'"
      ]
     },
     "execution_count": 2,
     "metadata": {},
     "output_type": "execute_result"
    }
   ],
   "source": [
    "pwd"
   ]
  },
  {
   "cell_type": "code",
   "execution_count": 4,
   "id": "7888e96b",
   "metadata": {},
   "outputs": [
    {
     "name": "stdout",
     "output_type": "stream",
     "text": [
      "/home/al2644/research/codebase/reasoning/perturb-r\n"
     ]
    }
   ],
   "source": [
    "cd /home/al2644/research/codebase/reasoning/perturb-r"
   ]
  },
  {
   "cell_type": "markdown",
   "id": "818fcb25",
   "metadata": {},
   "source": [
    "# Reasoning Results"
   ]
  },
  {
   "cell_type": "code",
   "execution_count": 80,
   "id": "88fa0269",
   "metadata": {
    "scrolled": false
   },
   "outputs": [
    {
     "name": "stdout",
     "output_type": "stream",
     "text": [
      "Qwen3-1.7B.pickle\n",
      "Pass@8 Accuracy: 0.6166666666666667\n",
      "Qwen3-1.7B_nothinking.pickle\n",
      "Pass@8 Accuracy: 0.2833333333333333\n",
      "Qwen3-8B.pickle\n",
      "Pass@8 Accuracy: 0.75\n",
      "Qwen3-8B_nothinking.pickle\n",
      "Pass@8 Accuracy: 0.4166666666666667\n"
     ]
    }
   ],
   "source": [
    "root = \"./results/aime2425/benchmark\"\n",
    "k = 8\n",
    "for fname in os.listdir(root):\n",
    "    if 'correct' not in fname:\n",
    "        print(fname)\n",
    "        df = pd.read_pickle(os.path.join(root, fname))\n",
    "        pass_at_k = df.groupby(\"problem\")[[\"correct\"]].max()[\"correct\"].mean()\n",
    "        print(f\"Pass@{k} Accuracy: {pass_at_k}\")"
   ]
  },
  {
   "cell_type": "code",
   "execution_count": 86,
   "id": "13482d0f",
   "metadata": {},
   "outputs": [],
   "source": [
    "df = pd.read_pickle(os.path.join(root, \"Qwen3-8B_nothinking.pickle\"))"
   ]
  },
  {
   "cell_type": "code",
   "execution_count": 97,
   "id": "ab66e3cf",
   "metadata": {},
   "outputs": [
    {
     "data": {
      "text/html": [
       "<div>\n",
       "<style scoped>\n",
       "    .dataframe tbody tr th:only-of-type {\n",
       "        vertical-align: middle;\n",
       "    }\n",
       "\n",
       "    .dataframe tbody tr th {\n",
       "        vertical-align: top;\n",
       "    }\n",
       "\n",
       "    .dataframe thead th {\n",
       "        text-align: right;\n",
       "    }\n",
       "</style>\n",
       "<table border=\"1\" class=\"dataframe\">\n",
       "  <thead>\n",
       "    <tr style=\"text-align: right;\">\n",
       "      <th></th>\n",
       "      <th>problem</th>\n",
       "      <th>solution</th>\n",
       "      <th>source</th>\n",
       "      <th>response</th>\n",
       "      <th>correct</th>\n",
       "    </tr>\n",
       "  </thead>\n",
       "  <tbody>\n",
       "    <tr>\n",
       "      <th>0</th>\n",
       "      <td>Let $x,y$ and $z$ be positive real numbers tha...</td>\n",
       "      <td>33</td>\n",
       "      <td>aime 24</td>\n",
       "      <td>We are given a system of logarithmic equations...</td>\n",
       "      <td>1.0</td>\n",
       "    </tr>\n",
       "    <tr>\n",
       "      <th>1</th>\n",
       "      <td>Let $x,y$ and $z$ be positive real numbers tha...</td>\n",
       "      <td>33</td>\n",
       "      <td>aime 24</td>\n",
       "      <td>We are given the system of equations:\\n\\n$$\\n\\...</td>\n",
       "      <td>1.0</td>\n",
       "    </tr>\n",
       "    <tr>\n",
       "      <th>2</th>\n",
       "      <td>Let $x,y$ and $z$ be positive real numbers tha...</td>\n",
       "      <td>33</td>\n",
       "      <td>aime 24</td>\n",
       "      <td>We are given three logarithmic equations invol...</td>\n",
       "      <td>0.0</td>\n",
       "    </tr>\n",
       "    <tr>\n",
       "      <th>3</th>\n",
       "      <td>Let $x,y$ and $z$ be positive real numbers tha...</td>\n",
       "      <td>33</td>\n",
       "      <td>aime 24</td>\n",
       "      <td>We are given the following system of equations...</td>\n",
       "      <td>1.0</td>\n",
       "    </tr>\n",
       "    <tr>\n",
       "      <th>4</th>\n",
       "      <td>Let $x,y$ and $z$ be positive real numbers tha...</td>\n",
       "      <td>33</td>\n",
       "      <td>aime 24</td>\n",
       "      <td>We are given the following system of logarithm...</td>\n",
       "      <td>1.0</td>\n",
       "    </tr>\n",
       "    <tr>\n",
       "      <th>...</th>\n",
       "      <td>...</td>\n",
       "      <td>...</td>\n",
       "      <td>...</td>\n",
       "      <td>...</td>\n",
       "      <td>...</td>\n",
       "    </tr>\n",
       "    <tr>\n",
       "      <th>475</th>\n",
       "      <td>There are exactly three positive real numbers ...</td>\n",
       "      <td>240</td>\n",
       "      <td>aime 25</td>\n",
       "      <td>We are given the function:\\n\\n$$\\nf(x) = \\frac...</td>\n",
       "      <td>0.0</td>\n",
       "    </tr>\n",
       "    <tr>\n",
       "      <th>476</th>\n",
       "      <td>There are exactly three positive real numbers ...</td>\n",
       "      <td>240</td>\n",
       "      <td>aime 25</td>\n",
       "      <td>We are given the function:\\n\\n$$\\nf(x) = \\frac...</td>\n",
       "      <td>0.0</td>\n",
       "    </tr>\n",
       "    <tr>\n",
       "      <th>477</th>\n",
       "      <td>There are exactly three positive real numbers ...</td>\n",
       "      <td>240</td>\n",
       "      <td>aime 25</td>\n",
       "      <td>We are given the function:\\n\\n$$\\nf(x) = \\frac...</td>\n",
       "      <td>0.0</td>\n",
       "    </tr>\n",
       "    <tr>\n",
       "      <th>478</th>\n",
       "      <td>There are exactly three positive real numbers ...</td>\n",
       "      <td>240</td>\n",
       "      <td>aime 25</td>\n",
       "      <td>We are given the function:\\n\\n$$\\nf(x) = \\frac...</td>\n",
       "      <td>0.0</td>\n",
       "    </tr>\n",
       "    <tr>\n",
       "      <th>479</th>\n",
       "      <td>There are exactly three positive real numbers ...</td>\n",
       "      <td>240</td>\n",
       "      <td>aime 25</td>\n",
       "      <td>We are given the function:\\n\\n$$\\nf(x) = \\frac...</td>\n",
       "      <td>0.0</td>\n",
       "    </tr>\n",
       "  </tbody>\n",
       "</table>\n",
       "<p>480 rows Ã— 5 columns</p>\n",
       "</div>"
      ],
      "text/plain": [
       "                                               problem solution   source  \\\n",
       "0    Let $x,y$ and $z$ be positive real numbers tha...       33  aime 24   \n",
       "1    Let $x,y$ and $z$ be positive real numbers tha...       33  aime 24   \n",
       "2    Let $x,y$ and $z$ be positive real numbers tha...       33  aime 24   \n",
       "3    Let $x,y$ and $z$ be positive real numbers tha...       33  aime 24   \n",
       "4    Let $x,y$ and $z$ be positive real numbers tha...       33  aime 24   \n",
       "..                                                 ...      ...      ...   \n",
       "475  There are exactly three positive real numbers ...      240  aime 25   \n",
       "476  There are exactly three positive real numbers ...      240  aime 25   \n",
       "477  There are exactly three positive real numbers ...      240  aime 25   \n",
       "478  There are exactly three positive real numbers ...      240  aime 25   \n",
       "479  There are exactly three positive real numbers ...      240  aime 25   \n",
       "\n",
       "                                              response  correct  \n",
       "0    We are given a system of logarithmic equations...      1.0  \n",
       "1    We are given the system of equations:\\n\\n$$\\n\\...      1.0  \n",
       "2    We are given three logarithmic equations invol...      0.0  \n",
       "3    We are given the following system of equations...      1.0  \n",
       "4    We are given the following system of logarithm...      1.0  \n",
       "..                                                 ...      ...  \n",
       "475  We are given the function:\\n\\n$$\\nf(x) = \\frac...      0.0  \n",
       "476  We are given the function:\\n\\n$$\\nf(x) = \\frac...      0.0  \n",
       "477  We are given the function:\\n\\n$$\\nf(x) = \\frac...      0.0  \n",
       "478  We are given the function:\\n\\n$$\\nf(x) = \\frac...      0.0  \n",
       "479  We are given the function:\\n\\n$$\\nf(x) = \\frac...      0.0  \n",
       "\n",
       "[480 rows x 5 columns]"
      ]
     },
     "execution_count": 97,
     "metadata": {},
     "output_type": "execute_result"
    }
   ],
   "source": [
    "df"
   ]
  },
  {
   "cell_type": "code",
   "execution_count": 39,
   "id": "f7d4a52c",
   "metadata": {},
   "outputs": [],
   "source": [
    "reasoning, answer = df[\"response\"][0].split(\"</think>\")"
   ]
  },
  {
   "cell_type": "code",
   "execution_count": 63,
   "id": "32ed62e0",
   "metadata": {},
   "outputs": [],
   "source": [
    "from utils.process_thinking import chunk as chunk_tool\n",
    "from reward_score.math import last_boxed_only_string, remove_boxed"
   ]
  },
  {
   "cell_type": "code",
   "execution_count": 69,
   "id": "5445b2ac",
   "metadata": {},
   "outputs": [],
   "source": [
    "chunks = chunk_tool(reasoning,30)\n",
    "final_answer = remove_boxed(last_boxed_only_string(reasoning))\n",
    "\n",
    "prompt = \"\"\n",
    "\n",
    "for idx, chunk in enumerate(chunks):\n",
    "    if final_answer not in chunk:\n",
    "        continue\n",
    "    prompt += f\"###START OF CHUNK {idx}\\n\"\n",
    "    prompt += chunk\n",
    "    prompt += f\"\\n###END OF CHUNK {idx}\\n\""
   ]
  },
  {
   "cell_type": "code",
   "execution_count": 70,
   "id": "111263ce",
   "metadata": {},
   "outputs": [],
   "source": [
    "instruction = \"\"\"<instruction>\n",
    "You are provided a chain of chunked model reasoning trace of deriving a solution to a problem. Your job is to identify where the answer is first reached in the reasoning chain and report the corresponding chunk number. The model may later verify or try alternative approach, but you should only focus on where the answer is first derived.\n",
    "\n",
    "You MUST include the chunk number inside <answer_chunk></answer_chunk>. This is a hard requirement for later processing.\n",
    "</instruction>\\n\\n\n",
    "The final answer is: 1\n",
    "\"\"\"\n",
    "input_str = instruction + prompt"
   ]
  },
  {
   "cell_type": "code",
   "execution_count": 72,
   "id": "203340ed",
   "metadata": {
    "scrolled": true
   },
   "outputs": [
    {
     "name": "stdout",
     "output_type": "stream",
     "text": [
      "<instruction>\n",
      "You are provided a chain of chunked model reasoning trace of deriving a solution to a problem. Your job is to identify where the answer is first reached in the reasoning chain and report the corresponding chunk number. The model may later verify or try alternative approach, but you should only focus on where the answer is first derived.\n",
      "\n",
      "You MUST include the chunk number inside <answer_chunk></answer_chunk>. This is a hard requirement for later processing.\n",
      "</instruction>\n",
      "\n",
      "\n",
      "The final answer is: 1\n",
      "###START OF CHUNK 0\n",
      "Okay, so I have this problem where I need to compute the asymptotic relative efficiency (ARE) for estimating \\( e^{-\\lambda} \\) in a Poisson process. The expression given is:\n",
      "\n",
      "\\[\n",
      "\\text{ARE} = \\left[\\frac{e^{-\\lambda}}{\\left(\\frac{n-1}{n}\\right)^{n\\lambda}\\log\\left( \\frac{n-1}{n}\\right)^n}\\right]^2\n",
      "\\]\n",
      "###END OF CHUNK 0\n",
      "###START OF CHUNK 3\n",
      "The numerator is \\( e^{-\\lambda} \\). The denominator has two main parts: \\( \\left(\\frac{n-1}{n}\\right)^{n\\lambda} \\) and \\( \\log\\left( \\frac{n-1}{n}\\right)^n \\).\n",
      "\n",
      "Wait, actually, the denominator is the entire expression \\( \\left(\\frac{n-1}{n}\\right)^{n\\lambda}\\log\\left( \\frac{n-1}{n}\\right)^n \\). So, it's the product of those two terms.\n",
      "###END OF CHUNK 3\n",
      "###START OF CHUNK 4\n",
      "Let me simplify the denominator step by step. First, \\( \\left(\\frac{n-1}{n}\\right)^{n\\lambda} \\). That looks similar to the limit definition of \\( e^{-\\lambda} \\) because \\( \\lim_{n \\to \\infty} \\left(1 - \\frac{1}{n}\\right)^n = e^{-1} \\), so \\( \\left(\\frac{n-1}{n}\\right)^{n} \\approx e^{-1} \\) for large \\( n \\). Similarly, \\( \\left(\\frac{n-1}{n}\\right)^{n\\lambda} = \\left(\\frac{n - 1}{n}\\right)^n \\cdot \\left(\\frac{n - 1}{n}\\right)^{\\lambda(n - 1)} \\). Hmm, maybe that's not the right approach.\n",
      "###END OF CHUNK 4\n",
      "###START OF CHUNK 5\n",
      "Wait, perhaps I can rewrite \\( \\left(\\frac{n-1}{n}\\right)^{n\\lambda} \\) as \\( \\left(1 - \\frac{1}{n}\\right)^{n\\lambda} \\). Similarly, \\( \\log\\left(\\frac{n-1}{n}\\right)^n = n \\log\\left(1 - \\frac{1}{n}\\right) \\). So, perhaps we can express everything in terms of \\( n \\) approaching infinity.\n",
      "###END OF CHUNK 5\n",
      "###START OF CHUNK 6\n",
      "Let me denote \\( p = \\frac{n - 1}{n} = 1 - \\frac{1}{n} \\). Then, \\( \\log\\left( \\frac{n - 1}{n} \\right)^n = n \\log p = n \\log\\left(1 - \\frac{1}{n}\\right) \\approx n \\left( -\\frac{1}{n} - \\frac{1}{2n^2} - \\cdots \\right) \\approx -1 - \\frac{1}{2n} - \\cdots \\) for large \\( n \\).\n",
      "###END OF CHUNK 6\n",
      "###START OF CHUNK 7\n",
      "Similarly, \\( \\left(\\frac{n - 1}{n}\\right)^{n\\lambda} = p^{n\\lambda} = \\left(1 - \\frac{1}{n}\\right)^{n\\lambda} \\approx e^{-\\lambda} \\left(1 + \\frac{\\lambda}{n} + \\cdots \\right) \\) for large \\( n \\).\n",
      "\n",
      "So, putting it together, the denominator is approximately \\( e^{-\\lambda} \\left(1 + \\frac{\\lambda}{n}\\right) \\times (-1 - \\frac{1}{2n}) \\). Let me compute that:\n",
      "\n",
      "Approximately, \\( e^{-\\lambda} \\times \\left(1 + \\frac{\\lambda}{n}\\right) \\times \\left(-1 - \\frac{1}{2n}\\right) \\).\n",
      "\n",
      "Multiplying these together:\n",
      "\n",
      "First, multiply \\( \\left(1 + \\frac{\\lambda}{n}\\right) \\) and \\( \\left(-1 - \\frac{1}{2n}\\right) \\):\n",
      "\n",
      "\\( 1 \\times (-1) = -1 \\)\n",
      "\n",
      "\\( 1 \\times (-\\frac{1}{2n}) = -\\frac{1}{2n} \\)\n",
      "\n",
      "\\( \\frac{\\lambda}{n} \\times (-1) = -\\frac{\\lambda}{n} \\)\n",
      "\n",
      "\\( \\frac{\\lambda}{n} \\times (-\\frac{1}{2n}) = -\\frac{\\lambda}{2n^2} \\)\n",
      "\n",
      "So, adding up the terms:\n",
      "\n",
      "\\( -1 - \\frac{1 + \\lambda}{2n} - \\frac{\\lambda}{2n^2} \\)\n",
      "\n",
      "For large \\( n \\), the higher order terms beyond \\( \\frac{1}{n} \\) become negligible, so approximately:\n",
      "\n",
      "\\( -1 - \\frac{1 + \\lambda}{2n} \\)\n",
      "\n",
      "Therefore, the denominator is approximately \\( e^{-\\lambda} \\times \\left(-1 - \\frac{1 + \\lambda}{2n}\\right) \\).\n",
      "\n",
      "Wait, but in the original expression, the denominator is \\( \\left(\\frac{n-1}{n}\\right)^{n\\lambda}\\log\\left( \\frac{n-1}{n}\\right)^n \\), which we approximated as \\( e^{-\\lambda} \\times \\left(-1 - \\frac{1 + \\lambda}{2n}\\right) \\).\n",
      "\n",
      "But hold on, \\( \\left(\\frac{n-1}{n}\\right)^{n\\lambda} \\) is approximately \\( e^{-\\lambda} \\), and \\( \\log\\left( \\frac{n-1}{n}\\right)^n \\) is approximately \\( -1 - \\frac{1}{2n} \\). So, multiplying these together:\n",
      "\n",
      "\\( e^{-\\lambda} \\times \\left(-1 - \\frac{1}{2n}\\right) \\).\n",
      "\n",
      "So, the denominator is approximately \\( -e^{-\\lambda} \\left(1 + \\frac{1}{2n}\\right) \\).\n",
      "\n",
      "Therefore, the denominator is approximately \\( -e^{-\\lambda} - \\frac{e^{-\\lambda}}{2n} \\).\n",
      "###END OF CHUNK 7\n",
      "###START OF CHUNK 9\n",
      "Wait, let me think again. The denominator is \\( \\left(\\frac{n-1}{n}\\right)^{n\\lambda}\\log\\left( \\frac{n-1}{n}\\right)^n \\). So, \\( \\left(\\frac{n-1}{n}\\right)^{n\\lambda} \\) is positive, and \\( \\log\\left( \\frac{n-1}{n}\\right)^n \\) is negative because \\( \\frac{n-1}{n} < 1 \\), so its logarithm is negative. Therefore, the denominator is positive multiplied by negative, so it's negative. But then the entire expression is \\( e^{-\\lambda} \\) divided by a negative number. That would make the whole expression negative, which can't be right because ARE is a positive number.\n",
      "\n",
      "So, perhaps I made a mistake in the sign somewhere. Let me double-check.\n",
      "###END OF CHUNK 9\n",
      "###START OF CHUNK 10\n",
      "Wait, \\( \\log\\left( \\frac{n-1}{n}\\right)^n = n \\log\\left(1 - \\frac{1}{n}\\right) \\approx -1 - \\frac{1}{2n} \\). That's correct because \\( \\log(1 - x) \\approx -x - x^2/2 \\) for small \\( x \\).\n",
      "###END OF CHUNK 10\n",
      "###START OF CHUNK 11\n",
      "And \\( \\left(\\frac{n - 1}{n}\\right)^{n \\lambda} = e^{n \\lambda \\log\\left(1 - \\frac{1}{n}\\right)} \\approx e^{n \\lambda (-1/n - 1/(2n^2))} \\approx e^{-\\lambda - \\lambda/(2n)} \\approx e^{-\\lambda} \\left(1 - \\frac{\\lambda}{2n}\\right) \\).\n",
      "\n",
      "So, the first term is \\( e^{-\\lambda} (1 - \\frac{\\lambda}{2n}) \\) and the second term is \\( -1 - \\frac{1}{2n} \\).\n",
      "\n",
      "Multiplying these together:\n",
      "\n",
      "\\( e^{-\\lambda} (1 - \\frac{\\lambda}{2n}) (-1 - \\frac{1}{2n}) \\approx e^{-\\lambda} [ -1 - \\frac{1}{2n} + \\frac{\\lambda}{2n} + \\frac{\\lambda}{4n^2} ] \\)\n",
      "\n",
      "Which simplifies to:\n",
      "\n",
      "\\( -e^{-\\lambda} - \\frac{e^{-\\lambda}}{2n} + \\frac{\\lambda e^{-\\lambda}}{2n} + \\cdots \\)\n",
      "\n",
      "So, approximately:\n",
      "\n",
      "\\( -e^{-\\lambda} + \\left( \\frac{\\lambda - 1}{2} e^{-\\lambda} \\right) \\frac{1}{n} \\)\n",
      "\n",
      "Therefore, the denominator is approximately \\( -e^{-\\lambda} + \\frac{(\\lambda - 1)e^{-\\lambda}}{2n} \\).\n",
      "\n",
      "So, the denominator is approximately \\( -e^{-\\lambda} \\) plus a small term.\n",
      "###END OF CHUNK 11\n",
      "###START OF CHUNK 12\n",
      "Therefore, the numerator is \\( e^{-\\lambda} \\), so the entire expression is \\( \\frac{e^{-\\lambda}}{-e^{-\\lambda} + \\cdots} \\approx \\frac{e^{-\\lambda}}{-e^{-\\lambda}} \\times \\left(1 - \\frac{(\\lambda - 1)e^{-\\lambda}}{2n} \\right) \\approx -1 + \\frac{(\\lambda - 1)e^{-\\lambda}}{2n} \\).\n",
      "###END OF CHUNK 12\n",
      "###START OF CHUNK 13\n",
      "But since ARE should be positive, perhaps I took the wrong approach. Maybe I need to consider the absolute value or perhaps the original expression is supposed to be an absolute value? Or maybe I need to reconsider the order of operations.\n",
      "\n",
      "Wait, let's look back at the original expression:\n",
      "\n",
      "\\[\n",
      "\\text{ARE} = \\left[\\frac{e^{-\\lambda}}{\\left(\\frac{n-1}{n}\\right)^{n\\lambda}\\log\\left( \\frac{n-1}{n}\\right)^n}\\right]^2\n",
      "\\]\n",
      "###END OF CHUNK 13\n",
      "###START OF CHUNK 14\n",
      "Since both numerator and denominator are positive or negative? The numerator is \\( e^{-\\lambda} \\) which is positive. The denominator is \\( \\left(\\frac{n-1}{n}\\right)^{n\\lambda} \\) which is positive, multiplied by \\( \\log\\left( \\frac{n-1}{n}\\right)^n \\) which is negative. So, the denominator is negative. Therefore, the entire expression is \\( \\frac{positive}{negative} \\), which is negative. But ARE is a positive number, so perhaps I missed an absolute value? Or maybe I need to take the reciprocal.\n",
      "###END OF CHUNK 14\n",
      "###START OF CHUNK 16\n",
      "Alternatively, perhaps the denominator is actually positive because \\( \\left(\\frac{n-1}{n}\\right)^{n\\lambda} \\) is positive, and \\( \\log\\left( \\frac{n-1}{n}\\right)^n \\) is negative, so the denominator is negative, but the numerator is positive, so the ratio is negative. But ARE is defined as the ratio of variances, which is positive, so maybe the absolute value is taken inside.\n",
      "###END OF CHUNK 16\n",
      "###START OF CHUNK 17\n",
      "Alternatively, perhaps I can think of it as:\n",
      "\n",
      "\\( \\text{ARE} = \\left[ \\frac{e^{-\\lambda}}{ \\left( \\frac{n-1}{n} \\right)^{n\\lambda} \\log \\left( \\frac{n-1}{n} \\right)^n } \\right]^2 \\)\n",
      "\n",
      "But since the expression inside is negative, squaring it would make it positive, but perhaps in the context of ARE, they take the absolute value.\n",
      "\n",
      "Alternatively, maybe I made a mistake in the approximation.\n",
      "\n",
      "Wait, let's think differently. Maybe I can write the denominator as \\( \\left( \\frac{n - 1}{n} \\right)^{n \\lambda} \\times \\log \\left( \\frac{n - 1}{n} \\right)^n \\).\n",
      "\n",
      "Let me denote \\( p = \\frac{n - 1}{n} = 1 - \\frac{1}{n} \\). So, \\( \\log p = \\log \\left(1 - \\frac{1}{n}\\right) \\approx -\\frac{1}{n} - \\frac{1}{2n^2} - \\cdots \\).\n",
      "###END OF CHUNK 17\n",
      "###START OF CHUNK 18\n",
      "Similarly, \\( \\left( \\frac{n - 1}{n} \\right)^{n \\lambda} = p^{n \\lambda} = e^{n \\lambda \\log p} \\approx e^{n \\lambda (-1/n - 1/(2n^2) - \\cdots)} = e^{-\\lambda - \\lambda/(2n) - \\cdots} \\approx e^{-\\lambda} \\left(1 - \\frac{\\lambda}{2n} + \\cdots \\right) \\).\n",
      "\n",
      "Therefore, the denominator is approximately \\( e^{-\\lambda} \\times \\left(-1 - \\frac{1}{2n}\\right) \\).\n",
      "###END OF CHUNK 18\n",
      "###START OF CHUNK 19\n",
      "So, putting it together, the expression inside the brackets is \\( \\frac{e^{-\\lambda}}{e^{-\\lambda} \\times \\left(-1 - \\frac{1}{2n}\\right)} = \\frac{1}{-1 - \\frac{1}{2n}} = -\\frac{1}{1 + \\frac{1}{2n}} \\approx -\\left(1 - \\frac{1}{2n} + \\frac{1}{4n^2} - \\cdots \\right) \\approx -1 + \\frac{1}{2n} \\).\n",
      "###END OF CHUNK 19\n",
      "###START OF CHUNK 20\n",
      "Therefore, the numerator is \\( e^{-\\lambda} \\), and the denominator is approximately \\( -e^{-\\lambda} + \\frac{e^{-\\lambda}}{2n} \\). Wait, hold on, no, because numerator is \\( e^{-\\lambda} \\), denominator is \\( e^{-\\lambda} \\times \\left(-1 - \\frac{1}{2n}\\right) \\). So, the ratio is \\( \\frac{e^{-\\lambda}}{e^{-\\lambda}(-1 - 1/(2n))} = \\frac{1}{-1 - 1/(2n)} \\approx -1 + 1/(2n) \\).\n",
      "\n",
      "So, squaring this, the ARE is \\( \\left(-1 + \\frac{1}{2n}\\right)^2 \\approx 1 - \\frac{1}{n} + \\frac{1}{4n^2} \\). As \\( n \\) approaches infinity, the ARE tends to 1.\n",
      "###END OF CHUNK 20\n",
      "###START OF CHUNK 21\n",
      "But that seems odd because ARE is supposed to be a measure of efficiency, and if the ARE is approaching 1, it suggests that the estimator is equally efficient as the other one as \\( n \\) becomes large.\n",
      "###END OF CHUNK 21\n",
      "###START OF CHUNK 22\n",
      "But wait, let's think again. Maybe I messed up the sign somewhere.\n",
      "\n",
      "Wait, in the denominator, it's \\( \\left(\\frac{n - 1}{n}\\right)^{n \\lambda} \\times \\log\\left( \\frac{n - 1}{n} \\right)^n \\). So, both terms are involved.\n",
      "###END OF CHUNK 22\n",
      "###START OF CHUNK 23\n",
      "But \\( \\log\\left( \\frac{n - 1}{n} \\right)^n = n \\log\\left(1 - \\frac{1}{n}\\right) \\approx -1 - \\frac{1}{2n} \\). So, the denominator is \\( \\left(\\frac{n - 1}{n}\\right)^{n \\lambda} \\times \\left(-1 - \\frac{1}{2n}\\right) \\).\n",
      "###END OF CHUNK 23\n",
      "###START OF CHUNK 24\n",
      "So, the denominator is approximately \\( e^{-\\lambda} \\times \\left(-1 - \\frac{1}{2n}\\right) \\). Therefore, the expression inside the brackets is \\( \\frac{e^{-\\lambda}}{e^{-\\lambda} \\times \\left(-1 - \\frac{1}{2n}\\right)} = \\frac{1}{-1 - \\frac{1}{2n}} \\approx -1 + \\frac{1}{2n} \\).\n",
      "###END OF CHUNK 24\n",
      "###START OF CHUNK 25\n",
      "So, squaring that, we have \\( \\left(-1 + \\frac{1}{2n}\\right)^2 = 1 - \\frac{1}{n} + \\frac{1}{4n^2} \\). So, as \\( n \\) becomes large, the ARE tends to 1, meaning both estimators are equally efficient in the limit.\n",
      "###END OF CHUNK 25\n",
      "###START OF CHUNK 31\n",
      "But in the expression given, it's a ratio between \\( e^{-\\lambda} \\) and another expression, which is \\( \\left(\\frac{n - 1}{n}\\right)^{n\\lambda}\\log\\left( \\frac{n - 1}{n}\\right)^n \\). So, perhaps that's the ratio of two estimators?\n",
      "###END OF CHUNK 31\n",
      "###START OF CHUNK 32\n",
      "Wait, maybe the numerator is an estimator for \\( e^{-\\lambda} \\) and the denominator is another estimator?\n",
      "\n",
      "Wait, but \\( e^{-\\lambda} \\) is the true value, so that would be 1 asymptotically. That can't be, so perhaps the expression is actually about the ratio of two estimators.\n",
      "###END OF CHUNK 32\n",
      "###START OF CHUNK 34\n",
      "Wait, unless that expression is the ratio of two estimators. So, perhaps \\( \\text{Estimator}_1 = e^{-\\lambda} \\) and \\( \\text{Estimator}_2 = \\left(\\frac{n - 1}{n}\\right)^{n\\lambda}\\log\\left( \\frac{n - 1}{n}\\right)^n \\). Then, ARE is the ratio of the variances.\n",
      "###END OF CHUNK 34\n",
      "###START OF CHUNK 35\n",
      "But if \\( \\text{Estimator}_1 = e^{-\\lambda} \\), which is a constant, not an estimator, but rather the true value, that doesn't make much sense because ARE requires both estimators to be estimators, i.e., random variables.\n",
      "###END OF CHUNK 35\n",
      "###START OF CHUNK 38\n",
      "But in the given expression, it's a ratio between \\( e^{-\\lambda} \\) and another term. Hmm, perhaps the ratio is \\( \\hat{\\theta} / \\hat{\\theta}' \\), and then squared.\n",
      "\n",
      "But without knowing what the other estimator is, it's hard to compute the ARE.\n",
      "\n",
      "Wait, looking back at the original expression:\n",
      "\n",
      "\\[\n",
      "\\text{ARE} = \\left[\\frac{e^{-\\lambda}}{\\left(\\frac{n-1}{n}\\right)^{n\\lambda}\\log\\left( \\frac{n-1}{n}\\right)^n}\\right]^2\n",
      "\\]\n",
      "\n",
      "So, the numerator is \\( e^{-\\lambda} \\), and the denominator is \\( \\left(\\frac{n - 1}{n}\\right)^{n\\lambda} \\times \\log\\left( \\frac{n - 1}{n}\\right)^n \\).\n",
      "###END OF CHUNK 38\n",
      "###START OF CHUNK 39\n",
      "If I think of \\( \\left(\\frac{n - 1}{n}\\right)^{n\\lambda} \\) as an estimator for \\( e^{-\\lambda} \\), then perhaps the denominator is another estimator, say \\( \\hat{\\theta}' = \\left(\\frac{n - 1}{n}\\right)^{n\\lambda} \\times \\log\\left( \\frac{n - 1}{n}\\right)^n \\).\n",
      "###END OF CHUNK 39\n",
      "###START OF CHUNK 46\n",
      "Wait, let's think in terms of the given expression: it's the square of \\( \\frac{e^{-\\lambda}}{\\text{something}} \\). So, if I denote \\( \\text{something} = \\left(\\frac{n - 1}{n}\\right)^{n\\lambda}\\log\\left( \\frac{n - 1}{n}\\right)^n \\), then the expression is \\( \\left( \\frac{e^{-\\lambda}}{\\text{something}} \\right)^2 \\).\n",
      "###END OF CHUNK 46\n",
      "###START OF CHUNK 47\n",
      "So, if I can figure out what \\( \\text{something} \\) is, perhaps I can get the ratio.\n",
      "\n",
      "Wait, \\( \\text{something} = \\left(\\frac{n - 1}{n}\\right)^{n\\lambda} \\times \\log\\left( \\frac{n - 1}{n} \\right)^n \\).\n",
      "\n",
      "Which is the same as \\( \\left(1 - \\frac{1}{n}\\right)^{n\\lambda} \\times \\log\\left(1 - \\frac{1}{n}\\right)^n \\).\n",
      "\n",
      "So, as \\( n \\) becomes large, \\( \\log\\left(1 - \\frac{1}{n}\\right)^n \\approx -1 - \\frac{1}{2n} \\). And \\( \\left(1 - \\frac{1}{n}\\right)^{n\\lambda} \\approx e^{-\\lambda} \\left(1 - \\frac{\\lambda}{n} \\right) \\).\n",
      "\n",
      "So, multiplying them together:\n",
      "\n",
      "\\( e^{-\\lambda} \\left(1 - \\frac{\\lambda}{n} \\right) \\times \\left(-1 - \\frac{1}{2n} \\right) \\approx e^{-\\lambda} \\left(-1 - \\frac{1}{2n} + \\frac{\\lambda}{n} + \\frac{\\lambda}{2n^2} \\right) \\).\n",
      "\n",
      "Which simplifies to:\n",
      "\n",
      "\\( -e^{-\\lambda} + \\left( -\\frac{1}{2} + \\lambda \\right) \\frac{e^{-\\lambda}}{n} + \\cdots \\).\n",
      "\n",
      "Therefore, \\( \\text{something} \\approx -e^{-\\lambda} + \\frac{ (\\lambda - 1/2)e^{-\\lambda} }{n} \\).\n",
      "\n",
      "Therefore, the ratio \\( \\frac{e^{-\\lambda}}{\\text{something}} \\approx \\frac{e^{-\\lambda}}{ -e^{-\\lambda} + \\frac{ (\\lambda - 1/2)e^{-\\lambda} }{n} } = \\frac{1}{-1 + \\frac{\\lambda - 1/2}{n} } \\approx -1 + \\frac{\\lambda - 1/2}{n} \\).\n",
      "\n",
      "Therefore, the ratio \\( \\frac{e^{-\\lambda}}{\\text{something}} \\approx -1 + \\frac{\\lambda - 1/2}{n} \\), and squaring it gives:\n",
      "\n",
      "\\( \\left( -1 + \\frac{\\lambda - 1/2}{n} \\right)^2 \\approx 1 - \\frac{2\\lambda - 1}{n} + \\frac{(\\lambda - 1/2)^2}{n^2} \\).\n",
      "\n",
      "Therefore, as \\( n \\) becomes large, the ARE tends to 1, meaning that both estimators are equally efficient.\n",
      "###END OF CHUNK 47\n",
      "###START OF CHUNK 48\n",
      "But this is under the assumption that \\( \\text{something} \\) is an estimator for \\( e^{-\\lambda} \\). But wait, \\( \\text{something} \\) is \\( \\left(\\frac{n - 1}{n}\\right)^{n\\lambda} \\times \\log\\left( \\frac{n - 1}{n} \\right)^n \\). So, if I think of \\( \\left(\\frac{n - 1}{n}\\right)^{n\\lambda} \\) as an estimator for \\( e^{-\\lambda} \\), and \\( \\log\\left( \\frac{n - 1}{n} \\right)^n \\) as a term, then perhaps it's not a standard estimator.\n",
      "###END OF CHUNK 48\n",
      "###START OF CHUNK 52\n",
      "But in that case, the numerator would be \\( \\hat{\\theta} = e^{-\\lambda} \\), and the denominator would be \\( \\hat{\\theta}' = \\left(\\frac{n - 1}{n}\\right)^{n\\lambda}\\log\\left( \\frac{n - 1}{n}\\right)^n \\). Therefore, the ARE is \\( \\left( \\frac{\\hat{\\theta}}{\\hat{\\theta}'} \\right)^2 \\).\n",
      "###END OF CHUNK 52\n",
      "###START OF CHUNK 53\n",
      "But then, in this case, \\( \\hat{\\theta}' \\) is an estimator for \\( e^{-\\lambda} \\times \\log\\left( \\frac{n - 1}{n} \\right)^n \\). Hmm, but \\( \\log\\left( \\frac{n - 1}{n} \\right)^n = n \\log\\left(1 - \\frac{1}{n}\\right) \\approx -1 - \\frac{1}{2n} \\). So, \\( \\hat{\\theta}' \\approx -e^{-\\lambda} \\left(1 + \\frac{1}{2n} \\right) \\). Therefore, \\( \\hat{\\theta}' \\approx -e^{-\\lambda} - \\frac{e^{-\\lambda}}{2n} \\).\n",
      "###END OF CHUNK 53\n",
      "###START OF CHUNK 54\n",
      "Therefore, the ratio \\( \\frac{\\hat{\\theta}}{\\hat{\\theta}'} \\approx \\frac{e^{-\\lambda}}{ -e^{-\\lambda} - \\frac{e^{-\\lambda}}{2n} } = \\frac{1}{ -1 - \\frac{1}{2n} } \\approx -1 + \\frac{1}{2n} \\).\n",
      "\n",
      "Therefore, the ratio squared is \\( \\left(-1 + \\frac{1}{2n}\\right)^2 \\approx 1 - \\frac{1}{n} + \\frac{1}{4n^2} \\), so as \\( n \\) tends to infinity, the ARE tends to 1.\n",
      "\n",
      "But again, this is speculative because I don't know what the other estimator is.\n",
      "\n",
      "Alternatively, maybe the given expression is the ratio of two estimators for \\( e^{-\\lambda} \\), each involving \\( \\lambda \\), and the ARE is the ratio of their variances.\n",
      "###END OF CHUNK 54\n",
      "###START OF CHUNK 55\n",
      "But in that case, we need to figure out what the two estimators are. Since the expression is given as a ratio, maybe \\( \\text{Estimator1} = e^{-\\lambda} \\) and \\( \\text{Estimator2} = \\left(\\frac{n - 1}{n}\\right)^{n\\lambda}\\log\\left( \\frac{n - 1}{n}\\right)^n \\), so ARE is \\( \\text{Var}(\\text{Estimator1}) / \\text{Var}(\\text{Estimator2}) \\).\n",
      "###END OF CHUNK 55\n",
      "###START OF CHUNK 56\n",
      "But in this case, \\( \\text{Estimator1} = e^{-\\lambda} \\) is a constant, not a random variable, so its variance would be zero, which can't be. So, perhaps I need to reinterpret.\n",
      "###END OF CHUNK 56\n",
      "###START OF CHUNK 58\n",
      "But in that case, both estimators should be functions of the same data, so perhaps the denominator is \\( \\left(\\frac{n - 1}{n}\\right)^{n\\lambda} \\times \\log\\left( \\frac{n - 1}{n} \\right)^n \\), which is the same as the numerator. So, that seems redundant.\n",
      "###END OF CHUNK 58\n",
      "###START OF CHUNK 61\n",
      "Wait, if I consider that \\( e^{-\\lambda} \\) is the true value, and we have two estimators \\( \\hat{\\theta}_1 \\) and \\( \\hat{\\theta}_2 \\), both related to \\( e^{-\\lambda} \\), then the ARE is \\( \\text{Var}(\\hat{\\theta}_1) / \\text{Var}(\\hat{\\theta}_2) \\).\n",
      "\n",
      "But if the given expression is \\( \\left( \\frac{e^{-\\lambda}}{\\text{something}} \\right)^2 \\), perhaps that is the ratio of two estimators for \\( e^{-\\lambda} \\).\n",
      "###END OF CHUNK 61\n",
      "###START OF CHUNK 62\n",
      "Wait, let me try to write the given expression as \\( \\left( \\frac{\\text{Estimator1}}{\\text{Estimator2}} \\right)^2 \\), where \\( \\text{Estimator1} = e^{-\\lambda} \\) and \\( \\text{Estimator2} = \\left(\\frac{n - 1}{n}\\right)^{n\\lambda}\\log\\left( \\frac{n - 1}{n} \\right)^n \\). But \\( \\text{Estimator1} \\) is a constant, so it's not an estimator.\n",
      "###END OF CHUNK 62\n",
      "###START OF CHUNK 63\n",
      "Alternatively, perhaps \\( \\text{Estimator1} = e^{-\\lambda} \\) and \\( \\text{Estimator2} = \\left(\\frac{n - 1}{n}\\right)^{n\\lambda} \\times \\log\\left( \\frac{n - 1}{n} \\right)^n \\). Then, the ratio is \\( \\frac{e^{-\\lambda}}{ \\left(\\frac{n - 1}{n}\\right)^{n\\lambda} \\times \\log\\left( \\frac{n - 1}{n} \\right)^n } \\), which is exactly the given expression.\n",
      "###END OF CHUNK 63\n",
      "###START OF CHUNK 64\n",
      "Therefore, in this case, \\( \\text{Estimator1} = e^{-\\lambda} \\) and \\( \\text{Estimator2} = \\left(\\frac{n - 1}{n}\\right)^{n\\lambda} \\times \\log\\left( \\frac{n - 1}{n} \\right)^n \\). So, the ARE is the squared ratio of these two estimators.\n",
      "###END OF CHUNK 64\n",
      "###START OF CHUNK 65\n",
      "But as we saw earlier, both \\( \\text{Estimator1} \\) and \\( \\text{Estimator2} \\) involve \\( \\lambda \\), so perhaps they are both functions of \\( \\lambda \\), but I'm not sure.\n",
      "###END OF CHUNK 65\n",
      "###START OF CHUNK 66\n",
      "Wait, if \\( \\text{Estimator1} = e^{-\\lambda} \\), then it's a function of \\( \\lambda \\), and \\( \\text{Estimator2} = \\left(\\frac{n - 1}{n}\\right)^{n\\lambda} \\times \\log\\left( \\frac{n - 1}{n} \\right)^n \\), which is also a function of \\( \\lambda \\) and \\( n \\).\n",
      "###END OF CHUNK 66\n",
      "###START OF CHUNK 67\n",
      "Therefore, the ARE is the ratio of the variances of these two estimators as \\( n \\) approaches infinity.\n",
      "\n",
      "So, maybe I can compute the variance of \\( \\text{Estimator1} \\) and the variance of \\( \\text{Estimator2} \\), and then take their ratio.\n",
      "\n",
      "But \\( \\text{Estimator1} = e^{-\\lambda} \\) is a constant, not a random variable, so its variance is zero. That can't be. So, perhaps I misinterpret the problem.\n",
      "###END OF CHUNK 67\n",
      "###START OF CHUNK 68\n",
      "Wait, another thought: perhaps the given expression is the ratio of two estimators for \\( e^{-\\lambda} \\), both of which are based on the same data. For example, \\( \\text{Estimator1} = e^{-\\lambda} \\) and \\( \\text{Estimator2} = \\left(\\frac{n - 1}{n}\\right)^{n\\lambda} \\times \\log\\left( \\frac{n - 1}{n} \\right)^n \\), but then \\( \\text{Estimator1} \\) is a constant and \\( \\text{Estimator2} \\) is a function involving \\( n \\). So, that doesn't make sense.\n",
      "###END OF CHUNK 68\n",
      "###START OF CHUNK 69\n",
      "Alternatively, maybe the given expression is the ratio of two estimators for \\( e^{-\\lambda} \\), both of which are based on \\( n \\). For example, \\( \\text{Estimator1} = e^{-\\lambda} \\) and \\( \\text{Estimator2} = \\left(\\frac{n - 1}{n}\\right)^{n\\lambda} \\times \\log\\left( \\frac{n - 1}{n} \\right)^n \\). But again, \\( \\text{Estimator1} \\) is a constant.\n",
      "###END OF CHUNK 69\n",
      "###START OF CHUNK 70\n",
      "Wait, maybe the problem is about the ratio of two estimators for \\( e^{-\\lambda} \\), both of which are functions of \\( n \\). For example, \\( \\text{Estimator1} = e^{-\\lambda} \\) and \\( \\text{Estimator2} = \\left(\\frac{n - 1}{n}\\right)^{n\\lambda} \\times \\log\\left( \\frac{n - 1}{n} \\right)^n \\). So, both are functions of \\( n \\), and the ARE is the ratio of their variances.\n",
      "###END OF CHUNK 70\n",
      "###START OF CHUNK 71\n",
      "But then, \\( \\text{Estimator1} = e^{-\\lambda} \\) is a constant, so its variance is zero. Therefore, the ARE would be undefined, as the variance of the numerator is zero.\n",
      "\n",
      "So, perhaps I'm missing something here.\n",
      "###END OF CHUNK 71\n",
      "###START OF CHUNK 72\n",
      "Alternatively, maybe the given expression is the ratio of two estimators for \\( e^{-\\lambda} \\), both of which are functions of \\( n \\). For example, \\( \\text{Estimator1} = e^{-\\lambda} \\) and \\( \\text{Estimator2} = \\left(\\frac{n - 1}{n}\\right)^{n\\lambda} \\times \\log\\left( \\frac{n - 1}{n} \\right)^n \\). So, as \\( n \\) increases, both estimators are functions of \\( n \\), and the ARE is the ratio of their variances.\n",
      "###END OF CHUNK 72\n",
      "###START OF CHUNK 73\n",
      "But again, \\( \\text{Estimator1} = e^{-\\lambda} \\) is a constant, so its variance is zero, which can't be. So, perhaps I need to consider that \\( \\text{Estimator1} \\) is \\( e^{-\\lambda} \\) and \\( \\text{Estimator2} \\) is \\( \\left(\\frac{n - 1}{n}\\right)^{n\\lambda} \\times \\log\\left( \\frac{n - 1}{n} \\right)^n \\), but \\( \\text{Estimator1} \\) is a constant, so it's not an estimator.\n",
      "###END OF CHUNK 73\n",
      "###START OF CHUNK 76\n",
      "Wait, another thought: perhaps the given expression is the ratio of two estimators for the parameter \\( \\lambda \\), such that one is \\( \\hat{\\theta} = e^{-\\lambda} \\) and the other is \\( \\hat{\\theta}' = \\left(\\frac{n - 1}{n}\\right)^{n\\lambda}\\log\\left( \\frac{n - 1}{n}\\right)^n \\). So, the ratio is \\( \\frac{\\hat{\\theta}}{\\hat{\\theta}'} \\), squared.\n",
      "###END OF CHUNK 76\n",
      "###START OF CHUNK 77\n",
      "But again, \\( \\hat{\\theta} \\) is a constant, so its variance is zero.\n",
      "\n",
      "Alternatively, maybe the problem is about an estimator for \\( e^{-\\lambda} \\) and an estimator for \\( \\lambda \\), and the ARE is the ratio of their variances.\n",
      "\n",
      "But in that case, the given expression is \\( \\left[ \\frac{e^{-\\lambda}}{\\text{something}} \\right]^2 \\), so perhaps it's the ratio of two estimators for \\( e^{-\\lambda} \\), each involving \\( \\lambda \\).\n",
      "\n",
      "Wait, perhaps \\( \\text{something} \\) is an estimator for \\( \\lambda \\), and \\( e^{-\\lambda} \\) is another estimator. But that doesn't make sense either.\n",
      "\n",
      "Alternatively, perhaps the expression is about the ratio of two estimators for \\( e^{-\\lambda} \\), both involving \\( n \\), such that the ARE is the ratio of their variances.\n",
      "\n",
      "But given that \\( e^{-\\lambda} \\) is a constant, I don't know.\n",
      "\n",
      "Wait, another approach: perhaps take the logarithm of the given expression.\n",
      "\n",
      "Taking the natural logarithm:\n",
      "\n",
      "\\[\n",
      "\\ln\\left( \\text{ARE} \\right) = 2 \\left( \\ln(e^{-\\lambda}) - \\ln\\left( \\left(\\frac{n - 1}{n}\\right)^{n\\lambda}\\log\\left( \\frac{n - 1}{n}\\right)^n \\right) \\right)\n",
      "\\]\n",
      "\n",
      "Simplify:\n",
      "\n",
      "\\[\n",
      "\\ln\\left( \\text{ARE} \\right) = 2 \\left( -\\lambda - \\left( n\\lambda \\ln\\left(1 - \\frac{1}{n}\\right) + \\ln\\left( \\log\\left( \\frac{n - 1}{n} \\right)^n \\right) \\right) \\right)\n",
      "\\]\n",
      "\n",
      "Simplify each term:\n",
      "###END OF CHUNK 77\n",
      "###START OF CHUNK 78\n",
      "1. \\( -\\lambda \\)\n",
      "2. \\( -n\\lambda \\ln\\left(1 - \\frac{1}{n}\\right) \\approx -n\\lambda \\left( -\\frac{1}{n} - \\frac{1}{2n^2} \\right) = \\lambda - \\frac{\\lambda}{2n} \\)\n",
      "3. \\( -\\ln\\left( \\log\\left( \\frac{n - 1}{n} \\right)^n \\right) = -n \\ln\\left( \\log\\left(1 - \\frac{1}{n}\\right) \\right) \\approx -n \\ln\\left( -\\frac{1}{n} - \\frac{1}{2n^2} \\right) \\approx -n \\ln\\left( -\\frac{1}{n} \\right) \\). Wait, but \\( \\log\\left(1 - \\frac{1}{n}\\right) \\) is negative, so logarithm of a negative number is undefined.\n",
      "###END OF CHUNK 78\n",
      "###START OF CHUNK 79\n",
      "Wait, that's a problem. The logarithm is of a negative number, which is not defined in real numbers.\n",
      "\n",
      "So, perhaps I made a mistake in simplifying the logarithm term. Let's re-examine.\n",
      "\n",
      "We have \\( \\log\\left( \\frac{n - 1}{n} \\right) = \\log\\left(1 - \\frac{1}{n}\\right) \\approx -\\frac{1}{n} - \\frac{1}{2n^2} - \\cdots \\). So, \\( \\log\\left( \\frac{n - 1}{n} \\right) \\) is negative.\n",
      "\n",
      "Therefore, \\( \\log\\left( \\frac{n - 1}{n} \\right)^n = n \\log\\left( \\frac{n - 1}{n} \\right) \\approx n \\left( -\\frac{1}{n} - \\frac{1}{2n^2} \\right) = -1 - \\frac{1}{2n} \\).\n",
      "\n",
      "Thus, \\( \\ln\\left( \\log\\left( \\frac{n - 1}{n} \\right)^n \\right) \\approx \\ln\\left( -1 - \\frac{1}{2n} \\right) \\). But the natural logarithm of a negative number is undefined in real numbers.\n",
      "\n",
      "Therefore, this approach leads to a problem because we're taking the logarithm of a negative number.\n",
      "\n",
      "Hmm, perhaps this suggests that the given expression is not well-defined for real numbers, which can't be.\n",
      "\n",
      "Wait, maybe I misapplied the logarithm. Let's think again.\n",
      "\n",
      "We have \\( \\log\\left( \\frac{n - 1}{n} \\right)^n = n \\log\\left( \\frac{n - 1}{n} \\right) \\), which is equal to \\( n \\log\\left(1 - \\frac{1}{n}\\right) \\).\n",
      "###END OF CHUNK 79\n",
      "###START OF CHUNK 80\n",
      "But \\( \\log(1 - x) \\) is approximately \\( -x - \\frac{x^2}{2} - \\cdots \\) for small \\( x \\), so in our case, \\( x = \\frac{1}{n} \\), so \\( \\log\\left(1 - \\frac{1}{n}\\right) \\approx -\\frac{1}{n} - \\frac{1}{2n^2} \\). Therefore, \\( n \\log\\left(1 - \\frac{1}{n}\\right) \\approx -1 - \\frac{1}{2n} \\).\n",
      "###END OF CHUNK 80\n",
      "###START OF CHUNK 81\n",
      "Therefore, \\( \\log\\left( \\frac{n - 1}{n} \\right)^n \\approx -1 - \\frac{1}{2n} \\), which is negative. Thus, \\( \\ln\\left( \\log\\left( \\frac{n - 1}{n} \\right)^n \\right) \\) is the logarithm of a negative number, which is undefined in real numbers.\n",
      "###END OF CHUNK 81\n",
      "###START OF CHUNK 83\n",
      "Wait, let me check the approximation again. \\( \\log\\left(1 - \\frac{1}{n}\\right) \\approx -\\frac{1}{n} - \\frac{1}{2n^2} \\), so multiplying by \\( n \\), we get \\( -1 - \\frac{1}{2n} \\). So, that seems correct.\n",
      "###END OF CHUNK 83\n",
      "###START OF CHUNK 84\n",
      "Therefore, \\( \\log\\left( \\frac{n - 1}{n} \\right)^n \\approx -1 - \\frac{1}{2n} \\), which is negative.\n",
      "\n",
      "Thus, taking the logarithm of a negative number is undefined in real analysis.\n",
      "\n",
      "So, this suggests that the given expression is not a valid expression because it leads to an undefined logarithm.\n",
      "\n",
      "Therefore, perhaps the original expression is incorrect, or I misinterpreted it.\n",
      "\n",
      "Alternatively, maybe the expression is supposed to be squared, so that the negative sign cancels out, but in that case, it's still undefined.\n",
      "###END OF CHUNK 84\n",
      "###START OF CHUNK 85\n",
      "Alternatively, perhaps the denominator is supposed to be \\( \\left( \\frac{n - 1}{n} \\right)^{n\\lambda} \\times \\log\\left( \\frac{n}{n - 1} \\right)^n \\), which would be positive because \\( \\log\\left( \\frac{n}{n - 1} \\right) = - \\log\\left( \\frac{n - 1}{n} \\right) \\), so the logarithm would be positive.\n",
      "\n",
      "Wait, let me compute that.\n",
      "###END OF CHUNK 85\n",
      "###START OF CHUNK 86\n",
      "If I take \\( \\log\\left( \\frac{n}{n - 1} \\right)^n = n \\log\\left(1 + \\frac{1}{n - 1}\\right) \\approx n \\times \\frac{1}{n - 1} = \\frac{n}{n - 1} \\approx 1 + \\frac{1}{n} \\).\n",
      "###END OF CHUNK 86\n",
      "###START OF CHUNK 87\n",
      "So, \\( \\log\\left( \\frac{n}{n - 1} \\right)^n \\approx 1 + \\frac{1}{n} \\), which is positive.\n",
      "\n",
      "Therefore, perhaps the original expression is supposed to be \\( \\left(\\frac{n - 1}{n}\\right)^{n\\lambda} \\times \\log\\left( \\frac{n}{n - 1} \\right)^n \\), which would be positive.\n",
      "\n",
      "But as written, it's \\( \\left(\\frac{n - 1}{n}\\right)^{n\\lambda} \\times \\log\\left( \\frac{n - 1}{n} \\right)^n \\), which is negative.\n",
      "\n",
      "So, the given expression is incorrect because it leads to an undefined logarithm.\n",
      "\n",
      "Therefore, maybe the expression is supposed to be squared, and the negative sign is just a result of the approximation, so the ratio is squared, and the negative goes away.\n",
      "###END OF CHUNK 87\n",
      "###START OF CHUNK 88\n",
      "Therefore, perhaps the correct expression should have been \\( \\left(\\frac{n - 1}{n}\\right)^{n\\lambda} \\times \\log\\left( \\frac{n}{n - 1} \\right)^n \\), which is positive, and the given expression is a typo or misinterpretation.\n",
      "###END OF CHUNK 88\n",
      "###START OF CHUNK 89\n",
      "Assuming that, then the ratio \\( \\frac{e^{-\\lambda}}{\\left(\\frac{n - 1}{n}\\right)^{n\\lambda} \\times \\log\\left( \\frac{n}{n - 1} \\right)^n} \\) squared would give the ARE.\n",
      "\n",
      "So, let's proceed with that assumption.\n",
      "\n",
      "Therefore, the numerator is \\( e^{-\\lambda} \\), and the denominator is \\( \\left(\\frac{n - 1}{n}\\right)^{n\\lambda} \\times \\log\\left( \\frac{n}{n - 1} \\right)^n \\).\n",
      "\n",
      "So, let's compute \\( \\frac{e^{-\\lambda}}{\\left(\\frac{n - 1}{n}\\right)^{n\\lambda} \\times \\log\\left( \\frac{n}{n - 1} \\right)^n} \\).\n",
      "\n",
      "First, compute \\( \\left(\\frac{n - 1}{n}\\right)^{n\\lambda} \\).\n",
      "\n",
      "We know that \\( \\left(1 - \\frac{1}{n}\\right)^n \\approx e^{-1} \\), so \\( \\left(\\frac{n - 1}{n}\\right)^{n\\lambda} \\approx e^{-\\lambda} \\left(1 - \\frac{\\lambda}{2} + \\cdots \\right) \\).\n",
      "\n",
      "Similarly, \\( \\log\\left( \\frac{n}{n - 1} \\right) = \\log\\left(1 + \\frac{1}{n - 1}\\right) \\approx \\frac{1}{n - 1} \\approx \\frac{1}{n} \\).\n",
      "\n",
      "Therefore, \\( \\log\\left( \\frac{n}{n - 1} \\right)^n \\approx \\frac{n}{n} = 1 \\).\n",
      "\n",
      "So, the denominator is approximately \\( e^{-\\lambda} \\times 1 = e^{-\\lambda} \\).\n",
      "\n",
      "Therefore, the ratio is \\( \\frac{e^{-\\lambda}}{e^{-\\lambda}} = 1 \\), so the square is 1.\n",
      "\n",
      "But again, that's only an approximation as \\( n \\) tends to infinity. Therefore, the ARE tends to 1.\n",
      "\n",
      "But this seems off because I'm not sure how the given expression is supposed to be interpreted.\n",
      "\n",
      "Alternatively, perhaps the given expression is supposed to be \\( \\left(\\frac{n - 1}{n}\\right)^{n\\lambda} \\times \\log\\left( \\frac{n - 1}{n} \\right)^n \\), which is negative, and the expression is squared.\n",
      "###END OF CHUNK 89\n",
      "###START OF CHUNK 90\n",
      "But in that case, as we saw earlier, the ratio is approximately \\( -1 + \\frac{\\lambda - 1/2}{n} \\), so the square is approximately \\( 1 - \\frac{1}{n} + \\frac{\\lambda - 1/2}{n^2} \\), leading to an ARE of 1 as \\( n \\) tends to infinity.\n",
      "###END OF CHUNK 90\n",
      "###START OF CHUNK 92\n",
      "Alternatively, maybe the given expression is the ratio of two estimators for \\( e^{-\\lambda} \\), such as \\( \\hat{\\theta}_1 = e^{-\\lambda} \\) and \\( \\hat{\\theta}_2 = \\left(\\frac{n - 1}{n}\\right)^{n\\lambda}\\log\\left( \\frac{n - 1}{n} \\right)^n \\), but as \\( \\hat{\\theta}_1 \\) is a constant, its variance is zero, which can't be.\n",
      "###END OF CHUNK 92\n",
      "###START OF CHUNK 93\n",
      "Alternatively, perhaps the given expression is the ratio of two estimators, each of which is a function of \\( n \\), such as \\( \\hat{\\theta}_1 = e^{-\\lambda} \\) and \\( \\hat{\\theta}_2 = \\left(\\frac{n - 1}{n}\\right)^{n\\lambda}\\log\\left( \\frac{n - 1}{n} \\right)^n \\), but again, \\( \\hat{\\theta}_1 \\) is a constant.\n",
      "###END OF CHUNK 93\n",
      "###START OF CHUNK 96\n",
      "Alternatively, perhaps the given expression is the ratio of two estimators for \\( e^{-\\lambda} \\), one of which is \\( e^{-\\lambda} \\) itself, and the other is \\( \\left(\\frac{n - 1}{n}\\right)^{n\\lambda}\\log\\left( \\frac{n - 1}{n} \\right)^n \\), but as previously, the second estimator is negative.\n",
      "###END OF CHUNK 96\n",
      "###START OF CHUNK 99\n",
      "Wait, let me think differently. Suppose I have two estimators for \\( e^{-\\lambda} \\), \\( \\hat{\\theta}_1 \\) and \\( \\hat{\\theta}_2 \\), both based on the same data. Then, the ARE is the ratio of their variances. So, if I can figure out what \\( \\hat{\\theta}_1 \\) and \\( \\hat{\\theta}_2 \\) are, I can compute the ARE.\n",
      "###END OF CHUNK 99\n",
      "###START OF CHUNK 100\n",
      "But the given expression is \\( \\left[ \\frac{e^{-\\lambda}}{\\left(\\frac{n - 1}{n}\\right)^{n\\lambda}\\log\\left( \\frac{n - 1}{n} \\right)^n} \\right]^2 \\). So, perhaps \\( \\hat{\\theta}_1 = e^{-\\lambda} \\) and \\( \\hat{\\theta}_2 = \\left(\\frac{n - 1}{n}\\right)^{n\\lambda}\\log\\left( \\frac{n - 1}{n} \\right)^n \\), but as \\( \\hat{\\theta}_1 \\) is a constant, it's not an estimator.\n",
      "###END OF CHUNK 100\n",
      "###START OF CHUNK 101\n",
      "Alternatively, perhaps the given expression is the ratio of two estimators, each involving \\( n \\), such that \\( \\hat{\\theta}_1 = e^{-\\lambda} \\) and \\( \\hat{\\theta}_2 = \\left(\\frac{n - 1}{n}\\right)^{n\\lambda}\\log\\left( \\frac{n - 1}{n} \\right)^n \\), but again, \\( \\hat{\\theta}_1 \\) is a constant.\n",
      "\n",
      "Given that, perhaps the given expression is actually the ratio of two estimators for \\( \\lambda \\), not for \\( e^{-\\lambda} \\).\n",
      "###END OF CHUNK 101\n",
      "###START OF CHUNK 106\n",
      "Wait, another thought: perhaps the given expression is the ratio of two estimators for \\( e^{-\\lambda} \\), both of which are functions of \\( n \\), but in the numerator, it's squared. So, perhaps the expression is \\( \\left( \\frac{\\hat{\\theta}_1}{\\hat{\\theta}_2} \\right)^2 \\), where \\( \\hat{\\theta}_1 \\) and \\( \\hat{\\theta}_2 \\) are estimators for \\( e^{-\\lambda} \\).\n",
      "\n",
      "But again, without knowing what \\( \\hat{\\theta}_1 \\) and \\( \\hat{\\theta}_2 \\) are, I can't compute the ARE.\n",
      "###END OF CHUNK 106\n",
      "###START OF CHUNK 108\n",
      "But in that case, the given expression is not in the form of the ratio of two estimators, but rather the ratio of a constant and another term.\n",
      "\n",
      "Given that, I think I need to conclude that I can't compute the ARE based on the given expression because it leads to an undefined logarithm.\n",
      "\n",
      "Therefore, perhaps the given expression is incorrect or misinterpreted.\n",
      "\n",
      "Alternatively, if I ignore the negative sign, perhaps the expression is \\( \\left(\\frac{n - 1}{n}\\right)^{n\\lambda} \\log\\left( \\frac{n - 1}{n} \\right)^n \\), which would be negative, but squared, so it's positive.\n",
      "\n",
      "So, perhaps the given expression is \\( \\left(\\frac{n - 1}{n}\\right)^{n\\lambda} \\log\\left( \\frac{n - 1}{n} \\right)^n \\), squared.\n",
      "###END OF CHUNK 108\n",
      "###START OF CHUNK 109\n",
      "But then, if we square it, we get \\( \\left( \\left(\\frac{n - 1}{n}\\right)^{n\\lambda} \\log\\left( \\frac{n - 1}{n} \\right)^n \\right)^2 \\), which is \\( \\left( \\frac{n - 1}{n}\\right)^{2n\\lambda} \\left( \\log\\left( \\frac{n - 1}{n} \\right)^n \\right)^2 \\).\n",
      "###END OF CHUNK 109\n",
      "###START OF CHUNK 115\n",
      "But if both are estimators for \\( e^{-\\lambda} \\), then if both are unbiased, the ARE is 1, but if they're biased, the ARE would be less than 1.\n",
      "\n",
      "But without knowing the specific estimators, it's hard to compute.\n",
      "\n",
      "Alternatively, perhaps the given expression is the ratio of two estimators for \\( e^{-\\lambda} \\), each involving \\( n \\), and the ARE is the ratio of their variances.\n",
      "\n",
      "So, perhaps:\n",
      "\n",
      "- Numerator: \\( \\hat{\\theta}_1 = e^{-\\lambda} \\) (constant)\n",
      "- Denominator: \\( \\hat{\\theta}_2 = \\left(\\frac{n - 1}{n}\\right)^{n\\lambda}\\log\\left( \\frac{n - 1}{n} \\right)^n \\)\n",
      "\n",
      "But then, as before, \\( \\hat{\\theta}_1 \\) is a constant, so its variance is zero.\n",
      "\n",
      "Alternatively, perhaps the numerator is \\( \\hat{\\theta}_1 = e^{-\\lambda} \\) and the denominator is \\( \\hat{\\theta}_2 = \\left(\\frac{n - 1}{n}\\right)^{n\\lambda}\\log\\left( \\frac{n}{n - 1} \\right)^n \\), which is positive.\n",
      "\n",
      "But in that case, the ratio is \\( \\frac{e^{-\\lambda}}{e^{-\\lambda}} = 1 \\), so the square is 1, leading to an ARE of 1.\n",
      "\n",
      "But in that case, the denominator is a biased estimator, but the ratio is 1, so the ARE is 1.\n",
      "\n",
      "But that seems too simplistic.\n",
      "###END OF CHUNK 115\n",
      "###START OF CHUNK 116\n",
      "Alternatively, perhaps the denominator is \\( \\left(\\frac{n - 1}{n}\\right)^{n\\lambda}\\log\\left( \\frac{n}{n - 1} \\right)^n \\), which is a biased estimator, so the ratio is 1, but the ARE is the ratio of the variances.\n",
      "###END OF CHUNK 116\n",
      "###START OF CHUNK 117\n",
      "Thus, if \\( \\hat{\\theta}_1 \\) is an unbiased estimator with variance \\( V_1 \\), and \\( \\hat{\\theta}_2 \\) is a biased estimator with variance \\( V_2 \\), then the ARE is \\( \\frac{V_1}{V_2} \\).\n",
      "\n",
      "But then, without knowing \\( V_1 \\) and \\( V_2 \\), I can't compute it.\n",
      "###END OF CHUNK 117\n",
      "###START OF CHUNK 119\n",
      "Therefore, I think I have to conclude that I can't compute the ARE based on the given expression because it leads to an undefined logarithm, and thus, the expression is incorrect or misinterpreted.\n",
      "\n",
      "**Final Answer**\n",
      "\\boxed{1}\n",
      "\n",
      "###END OF CHUNK 119\n",
      "\n"
     ]
    }
   ],
   "source": [
    "print(input_str)"
   ]
  }
 ],
 "metadata": {
  "kernelspec": {
   "display_name": "Python 3 (ipykernel)",
   "language": "python",
   "name": "python3"
  },
  "language_info": {
   "codemirror_mode": {
    "name": "ipython",
    "version": 3
   },
   "file_extension": ".py",
   "mimetype": "text/x-python",
   "name": "python",
   "nbconvert_exporter": "python",
   "pygments_lexer": "ipython3",
   "version": "3.10.16"
  }
 },
 "nbformat": 4,
 "nbformat_minor": 5
}
